code/bignum/Hacl.Bignum.DefinitionsPulse.fst
@@ -35,3 +35,23 @@ let lbignum_pts_to #t #len (x: lbignum t len) (#[full_default()] f : perm) (v: S
 [@@pulse_unfold]
 instance lbignum_pts_to_inst #t #len : has_pts_to (lbignum t len) (S.lbignum t (v len)) =
   { pts_to = lbignum_pts_to }
+
+// TODO move to pulse
+fn arrayptr_memset (#t: Type0) (r: AP.ptr t) (x: t) (sz: SizeT.t)
+  requires exists* vr. pts_to r vr ** pure (Seq.length vr == SizeT.v sz)
+  ensures pts_to r (Seq.create (SizeT.v sz) x)
+{
+  let mut i = 0sz;
+  while (let vi = !i; SizeT.lt vi sz)
+    invariant b. exists* vi vr.
+      pts_to i vi ** pts_to r vr **
+      pure (SizeT.v vi <= SizeT.v sz /\ Seq.length vr == SizeT.v sz /\
+        (forall (j: nat). j < SizeT.v vi ==> Seq.index vr j == x)) **
+      pure (b == (SizeT.lt vi sz))
+  {
+    let vi = !i;
+    AP.(r.(vi) <- x);
+    i := SizeT.add vi 1sz;
+  };
+  with vr. assert pts_to r vr ** pure (vr `Seq.equal` Seq.create (SizeT.v sz) x);
+}
