code/bignum/Hacl.Bignum.MultiplicationPulse.fst
@@ -10,6 +10,7 @@ open Hacl.Impl.LibPulse
 
 module LSeq = Lib.Sequence
 module S = Hacl.Spec.Bignum.Multiplication
+module SD = Hacl.Spec.Bignum.Definitions
 module SS = Hacl.Spec.Bignum.Squaring
 module SL = Hacl.Spec.Lib
 module AP = Pulse.Lib.ArrayPtr
@@ -26,7 +27,7 @@ fn bn_mul1
   (a:lbignum t aLen)
   (l:limb t)
   (res:lbignum t aLen)
-  (#va: (SD.lbignum t (v aLen)))
+  (#va: erased (SD.lbignum t (v aLen)))
   requires pts_to a (va)
   requires exists* res0. pts_to res res0
   returns c_out: limb t
@@ -60,9 +61,10 @@ fn bn_mul1_add_in_place
   (a:lbignum t aLen)
   (l:limb t)
   (res:lbignum t aLen)
-  #va
+  (#va: erased (SD.lbignum t (v aLen)))
+  (#vres: erased (SD.lbignum t (v aLen)))
   requires pts_to a va
-  requires exists* vres. pts_to res vres
+  requires pts_to res vres
   returns c_out: limb t
   ensures pts_to a va
   ensures pts_to res (snd (S.bn_mul1_add_in_place va l vres))
@@ -71,7 +73,8 @@ fn bn_mul1_add_in_place
   let mut c = (uint #t 0 <: limb t);
 
   with body_ty. assert pure (body_ty ==
-    fill_elems_impl_ty aLen res (S.bn_mul1_add_in_place_f va l vres)
+    fill_elems_impl_ty aLen res #(fun j x -> x == Seq.index vres j)
+      (S.bn_mul1_add_in_place_f va l vres)
       fun i x -> pts_to c x ** pts_to a va);
   fn body () : body_ty = i #vr #vo {
     let a_i = AP.(a.(sizet_of_size_t i));
@@ -96,19 +99,24 @@ fn bn_mul1_lshift_add
   (resLen:size_t)
   (j:size_t{v j + v aLen <= v resLen})
   (res:lbignum t resLen)
-  #va
-  #vres
+  (#va: erased (SD.lbignum t (v aLen)))
+  (#vres: erased (SD.lbignum t (v resLen)))
   requires pts_to a va
-  requires exists* res_vres. pts_to res res_vres
+  requires pts_to res vres
   returns c_out: limb t
   ensures pts_to a va
-  ensures pts_to res (snd (S.bn_mul1_lshift_add va b_j (v j) res_vres))
-  ensures pure (c_out == fst (S.bn_mul1_lshift_add va b_j (v j) res_vres))
+  ensures pts_to res (snd (S.bn_mul1_lshift_add va b_j (v j) vres))
+  ensures pure (c_out == fst (S.bn_mul1_lshift_add va b_j (v j) vres))
 {
   let res_j = AP.split res (sizet_of_size_t j);
-  let res0: lbignum t aLen = coerce_eq () res_j; rewrite each res_j as res0;
-  let c_out = bn_mul1_add_in_place aLen a b_j res0;
-  AP.join res_j res; rewrite each res_j as res;
+  let res_rest = AP.ghost_split res_j (sizet_of_size_t aLen);
+  with vres_j. assert AP.pts_to res_j vres_j;
+  let c_out = bn_mul1_add_in_place aLen a b_j res_j;
+  AP.join res_j res_rest;
+  AP.join res res_j;
+  with vres'. assert pts_to res vres';
+  LSeq.lemma_update_sub' #(limb t) #(v resLen) vres (v j) (v aLen)
+    (snd (S.bn_mul1_add_in_place va b_j vres_j)) vres';
   c_out
 }
 
@@ -119,23 +127,33 @@ let bn_mul_st (t:limb_t) =
   -> bLen:size_t{v aLen + v bLen <= max_size_t}
   -> b:lbignum t bLen
   -> res:lbignum t (aLen +! bLen)
-  -> #va: _
-  -> #vb: _
-  -> #vres: _
+  -> #va: erased (SD.lbignum t (v aLen))
+  -> #vb: erased (SD.lbignum t (v bLen))
+  -> #vres: erased (SD.lbignum t (v (aLen +! bLen)))
   -> stt unit
   (requires pts_to a va ** pts_to b vb ** pts_to res vres)
-  (ensures fun _ -> pts_to a va ** pts_to b vb ** pts_to res (S.bn_mul va vb))
+  (ensures fun _ -> pts_to a va ** pts_to b vb ** lbignum_pts_to res (S.bn_mul va vb))
 
 inline_for_extraction noextract
 fn bn_mul (#t:limb_t) : bn_mul_st t = aLen a bLen b res #va #vb #vres {
-  memset res (uint #t 0) (aLen +! bLen);
-  let h0 = ST.get () in
-  fill_elems4 bLen res _ _ 
-  (fun j ->
-    let bj = AP.(b.(sizet_of_size_t j));
-    let c0 = bn_mul1_lshift_add aLen a bj (aLen +! bLen) j res;
-    c0
-  )
+  arrayptr_memset res (uint #t 0) (sizet_of_size_t (aLen +! bLen));
+  with vres0. assert pts_to res vres0;
+  let mut j = 0ul;
+  Lib.LoopCombinators.eq_repeati0 0 (S.bn_mul_ va vb) vres0;
+  while (let vj = !j; lt vj bLen)
+    invariant cond. exists* vj (vres : SD.lbignum t (v (aLen +! bLen))).
+      pts_to j vj ** pts_to res vres ** pts_to b vb ** pts_to a va **
+      pure (cond == lt vj bLen) **
+      pure (v vj <= v bLen /\
+        vres == Lib.LoopCombinators.repeati (v vj) (S.bn_mul_ va vb) vres0)
+  {
+    let vj = !j;
+    j := add vj 1ul;
+    let bj = AP.(b.(sizet_of_size_t vj));
+    let c0 = bn_mul1_lshift_add aLen a bj (aLen +! bLen) vj res;
+    Lib.LoopCombinators.unfold_repeati (v vj + 1) (S.bn_mul_ va vb) vres0 (v vj);
+    AP.(res.(sizet_of_size_t (aLen +! vj)) <- c0);
+  }
 }
 
 [@CInline]
@@ -155,20 +173,30 @@ fn bn_sqr_diag
   (aLen:size_t{v aLen + v aLen <= max_size_t})
   (a:lbignum t aLen)
   (res:lbignum t (aLen +! aLen))
-  #va
-  #vres
+  (#va: erased (SD.lbignum t (v aLen)))
   requires pts_to a va
-  requires pts_to res vres
-  ensures pts_to res (SS.bn_sqr_diag va)
+  requires lbignum_pts_to res (Seq.create #(limb t) (v aLen + v aLen) (uint #t 0))
+  ensures pts_to res (SS.bn_sqr_diag va <: SD.lbignum t (v (aLen +! aLen)))
   ensures pts_to a va
 {
-  let h0 = ST.get () in
-  fill_elems4 aLen res _ _ 
-  (fun i ->
-    let (hi, lo) = mul_wide (AP.(a.(sizet_of_size_t i))) (AP.(a.(sizet_of_size_t i)));
-    AR.to_array_ptr res (2ul *! i) lo;
-    AR.to_array_ptr res ((2ul *! i) +! 1ul) hi;
-  )
+  with vres0. assert pts_to res vres0;
+  let mut j = 0ul;
+  Lib.LoopCombinators.eq_repeati0 0 (SS.bn_sqr_diag_f va) vres0;
+  while (let vj = !j; lt vj aLen)
+    invariant cond. exists* vj (vres : SD.lbignum t (v (aLen +! aLen))).
+      pts_to j vj ** pts_to res vres ** pts_to a va **
+      pure (cond == lt vj aLen) **
+      pure (v vj <= v aLen /\
+        vres == Lib.LoopCombinators.repeati (v vj) (SS.bn_sqr_diag_f va) vres0)
+  {
+    let vj = !j;
+    let a_j = AP.(a.(sizet_of_size_t vj));
+    let (hi, lo) = mul_wide a_j a_j;
+    AP.(res.(sizet_of_size_t (2ul *! vj)) <- lo);
+    AP.(res.(sizet_of_size_t (2ul *! vj +! 1ul)) <- hi);
+    Lib.LoopCombinators.unfold_repeati (v vj + 1) (SS.bn_sqr_diag_f va) vres0 (v vj);
+    j := add vj 1ul;
+  }
 }
 
 inline_for_extraction noextract
@@ -176,30 +204,49 @@ let bn_sqr_st (t:limb_t) =
     aLen:size_t{0 < v aLen /\ v aLen + v aLen <= max_size_t}
   -> a:lbignum t aLen
   -> res:lbignum t (aLen +! aLen)
-  -> #va: _
-  -> #vres: _
+  -> #va: erased (SD.lbignum t (v aLen))
+  -> #vres: erased (SD.lbignum t (v (aLen +! aLen)))
   -> stt unit
   (requires pts_to a va ** pts_to res vres)
-  (ensures fun _ -> pts_to a va ** pts_to res (SS.bn_sqr va))
+  (ensures fun _ -> pts_to a va ** pts_to res (SS.bn_sqr va <: SD.lbignum t (v (aLen +! aLen))))
 
 inline_for_extraction noextract
 fn bn_sqr (#t:limb_t) : bn_sqr_st t = aLen a res #va #vres {
-  memset res (uint #t 0) (aLen +! aLen);
-  
-  fill_elems4 aLen res _ _ 
-  (fun j ->
-    let ab = AP.split a (sizet_of_size_t j);
-    let a_j = AP.(a.(sizet_of_size_t j));
-    let c0 = bn_mul1_lshift_add j ab a_j (aLen +! aLen) j res;
-    let res_v = SS.bn_sqr_diag va in
-    res_v
-  );
+  with resLen. assert (pure (resLen == aLen +! aLen));
+  arrayptr_memset res (uint #t 0) (sizet_of_size_t resLen);
+  with vres0. assert pts_to res vres0;
 
-  let tmp = create (aLen +! aLen) (uint #t 0) in
+  let mut j = 0ul;
+  with spec. assert pure (spec == SS.bn_sqr_f va);
+  Lib.LoopCombinators.eq_repeati0 0 spec vres0;
+  while (let vj = !j; lt vj aLen)
+    invariant cond. exists* vj (vres : SD.lbignum t (v (aLen +! aLen))).
+      pts_to j vj ** pts_to res vres ** pts_to a va **
+      pure (cond == lt vj aLen) **
+      pure (v vj <= v aLen /\
+        vres == Lib.LoopCombinators.repeati (v vj) spec vres0)
+  {
+    let vj = !j;
+    let a_j = AP.(a.(sizet_of_size_t vj));
+    let a_rest = AP.ghost_split a (sizet_of_size_t vj);
+    let ab: lbignum t vj = coerce_eq () a; rewrite each a as ab;
+    let res_v = bn_mul1_lshift_add vj ab a_j resLen vj res;
+    AP.join ab a_rest; rewrite each ab as a; with va'. assert pts_to a va' ** pure (Seq.equal va' va);
+    Lib.LoopCombinators.unfold_repeati (v vj + 1) spec vres0 (v vj);
+    AP.(res.(sizet_of_size_t (vj +! vj)) <- res_v);
+    j := add vj 1ul;
+  };
+
+  let _ = Hacl.Bignum.AdditionPulse.bn_dbl resLen res;
+
+  let mut tmp_arr = [| (uint #t 0 <: limb t); sizet_of_size_t (aLen +! aLen) |];
+  let tmp = AP.from_array tmp_arr;
   bn_sqr_diag aLen a tmp;
-  let c1 = Hacl.Bignum.AdditionPulse.bn_add_eq_len (aLen +! aLen) res tmp res in
-  ignore c1;
-  ()
+  with vtmp. assert AP.pts_to tmp vtmp;
+
+  let _ = Hacl.Bignum.AdditionPulse.bn_add_eq_len_inplace (aLen +! aLen) tmp res;
+
+  AP.to_array tmp _ #_ #vtmp;
 }
 
 [@CInline]
